Progress I guess.

circular-array-2.dfy
@@ -2,73 +2,124 @@
   Class CircularArray.
 */
 class {:autocontracts} CircularArray {
-    /*
-      Implementation
-    */
-    var a: array<int>; // The array.
-    var startIndex: nat; // The index of the first element.
-    var currentIndex: nat; // The index to put the next element.
-    var count: nat; // The number of elements.
+  /*
+    Implementation
+  */
+  var a: array<int>; // The array.
+  var startIndex: nat; // The index of the first element.
+  var currentIndex: nat; // The index to put the next element.
+  var count: nat; // The number of elements in the queue.
 
-    /*
-      Abstraction.
-    */
-    ghost var Elements: seq<int>; // The elements in the array represented as a sequence.
+  /*
+    Abstraction.
+  */
+  ghost var Elements: seq<int>; // The elements in the array represented as a sequence.
 
-    /*
-      Class invariant.
-    */
-    ghost predicate Valid()
-    {
-        0 <= startIndex <= a.Length &&
-        0 <= currentIndex <= a.Length &&
-        0 <= count <= a.Length &&
-        count == |Elements| &&
-        forall i: nat :: 0 <= i < count ==> Elements[i] == a[(startIndex + i) % a.Length]
+  /*
+    Class invariant.
+  */
+  ghost predicate Valid()
+  {
+    a.Length > 0 &&
+    0 <= startIndex < a.Length &&
+    0 <= currentIndex < a.Length &&
+    0 <= count <= a.Length &&
+    count == |Elements| &&
+    forall i :: 0 <= i < count ==> Elements[i] == a[(startIndex + i) % a.Length]
+  }
+
+  /*
+    Constructor.
+  */
+  constructor EmptyQueue()
+    ensures Valid()
+  {
+    a := new int[10];
+    startIndex := 0;
+    currentIndex := 0;
+    count := 0;
+    Elements := [];
+  }
+
+  /*
+    Enqueue method.
+  */
+  method Enqueue(element: int)
+    requires Valid()
+    ensures Valid()
+    ensures Elements == old(Elements) + [element]
+  {
+    if (count == a.Length) {
+      /*
+        Size limit reached, create a bigger array and transfer the elements.
+      */
+      var newA := new int[a.Length + 10];
+      var i := 0;
+      while (i < a.Length)
+        decreases a.Length - i
+        invariant 0 <= i <= a.Length < newA.Length
+        invariant forall j :: (0 <= j < i) ==> (a[(j + startIndex) % a.Length] == newA[j])
+      {
+        newA[i] := a[(i + startIndex) % a.Length];
+        i := i + 1;
+      }
+      /*
+        Update the fields.
+      */
+      a := newA;
+      startIndex := 0;
+      currentIndex := count;
     }
-
     /*
-      Constructor.
+      Go back to the beginning of the array if the end is reached.
     */
-    constructor WithInitialCapacity(capacity: nat)
-        requires capacity > 0
-        ensures Valid()
-    {
-        a := new int[capacity];
-        startIndex := 0;
-        currentIndex := 0;
-        count := 0;
-        Elements := [];
+    if (currentIndex >= a.Length) {
+      currentIndex := 0;
     }
-
     /*
-      Contains method.
+      Add the element to the array.
     */
-    method Contains(element: int) returns (r: bool)
-        requires Valid()
-        ensures Valid()
-        ensures r == (element in Elements)
-    {
-        r := false;
-        var i := 0;
-        while i < count
-            invariant 0 <= i <= count
-            invariant r == (element in Elements[0..i])
-            decreases count - i
-        {
-            if (a[(startIndex + i) % a.Length] == element) {
-                r := true;
-            }
-            i := i + 1;
-        }
-    }
-
+    a[currentIndex] := element;
+    currentIndex := currentIndex + 1;
+    count := count + 1;
     /*
-        Size function.
+      Update the abstraction.
     */
-    function Size(): nat
-        ensures Size() == count
-    {
-        count
-    }
+    Elements := Elements + [element];
+  }
+
+  /*
+    Contains method.
+  */
+  // method Contains(element: int) returns (r: bool)
+  //   requires Valid()
+  //   ensures Valid()
+  //   ensures r == (element in Elements)
+  // {
+  //   var s: seq<int> := [];
+  //   if (startIndex < currentIndex) {
+  //     s := a[startIndex..currentIndex];
+  //   } else {
+  //     s := a[startIndex..a.Length] + a[0..currentIndex];
+  //   }
+  //   r := element in s;
+  // }
+
+  /*
+    Size function.
+  */
+  function Size(): nat
+    ensures Size() == count
+  {
+    count
+  }
+
+  /*
+    IsEmpty function.
+  */
+  function IsEmpty(): bool
+    ensures IsEmpty() == (count == 0)
+  {
+    count == 0
+  }
 }
